monads/Monad.v
@@ -4,21 +4,22 @@ Module Type Monad.
   Parameter m : Type -> Type.
 
   (** "return" *)
-  Parameter ret : forall a, a -> m a.
+  Parameter ret : forall (A : Type), A -> m A.
+
   (** ">>=" *)
-  Parameter bind : forall a b, m a -> (a -> m b) -> m b.
+  Parameter bind : forall (A B : Type), m A -> (A -> m B) -> m B.
 
   (** Three laws that a monad instance must obey.
     Law 1:  return x >>= f ~ f x
     Law 2:  m >>= return ~ m
     Law 3:  (m >>= f) >>= g ~ m >>= (fun x -> f x >>= g) *)
-  Axiom monad_law1 : forall a b (x : a) (f : a -> m b),
+  Axiom monad_law1 : forall (A B : Type) (x : A) (f : A -> m B),
     bind (ret x) f = f x.
 
-  Axiom monad_law2 : forall a (x : m a),
-    bind x (@ret a) = x.
+  Axiom monad_law2 : forall (A : Type) (x : m A),
+    bind x (@ret A) = x.
 
-  Axiom monad_law3 : forall a b c (n : m a) (f : a -> m b) (g : b -> m c),
-    bind (bind n f) g = bind n (fun x => bind (f x) g).
-
+  Axiom monad_law3 :
+    forall (A B C : Type) (n : m A) (f : A -> m B) (g : B -> m C),
+      bind (bind n f) g = bind n (fun x => bind (f x) g).
 End Monad.
